IdSimClight extension

driver/ClightStep.v
@@ -23,73 +23,6 @@ Set Implicit Arguments.
 
 Local Opaque Z.mul Z.add Z.sub Z.div.
 
-
-
-Lemma ccc_id
-      (ccc: Csyntax.program)
-  :
-    exists mp,
-      (<<SIM: @ModPair.sim SimMemId.SimMemId SimMemId.SimSymbId SoundTop.Top mp>>)
-      /\ (<<SRC: mp.(ModPair.src) = ccc.(module)>>)
-      /\ (<<TGT: mp.(ModPair.tgt) = ccc.(module)>>)
-.
-Proof.
-  eexists (ModPair.mk _ _ _); s.
-  esplits; eauto. instantiate (1:=tt).
-  econs; ss; i.
-  rewrite SIMSKENVLINK in *.
-  eapply match_states_sim; ss.
-  - apply unit_ord_wf.
-  - eapply SoundTop.sound_state_local_preservation.
-  - instantiate (1:= fun sm_arg _ st_src st_tgt sm0 =>
-                       (<<EQ: st_src = st_tgt>>) /\
-                       (<<MWF: sm0.(SimMemId.src) = sm0.(SimMemId.tgt)>>) /\
-                       (<<STMWF: match st_src.(CsemC.get_mem) with
-                                 | Some m => sm0.(SimMemId.src) = m
-                                 | _ => True
-                                 end>>)).
-    ss. i.
-    destruct args_src, args_tgt, sm_arg. inv SIMARGS; ss; clarify.
-    clear SAFESRC. dup INITTGT. inv INITTGT. ss.
-    eexists. eexists (SimMemId.mk tgt tgt). esplits; eauto; ss.
-  - ii. destruct args_src, args_tgt, sm_arg. inv SIMARGS; ss; clarify.
-  - ii. ss. des. clarify.
-  - i. ss. des. clarify. esplits; eauto.
-    + inv CALLSRC. ss. clarify.
-    + instantiate (1:=top4). ss.
-  - i. clear HISTORY. ss. destruct sm_ret, retv_src, retv_tgt.
-    inv SIMRET. des. ss. clarify. eexists (SimMemId.mk _ _). esplits; eauto.
-    inv AFTERSRC. ss.
-  - i. ss. des. destruct sm0. ss. clarify. eexists (SimMemId.mk tgt tgt).
-    esplits; eauto.
-    inv FINALSRC. ss.
-  - right. ii. des. destruct sm0. ss. clarify. esplits; eauto.
-    + i. exploit H; ss.
-      * econs 1.
-      * i. des; clarify. econs; eauto.
-    + i. exists tt, st_tgt1.
-      exists (match st_tgt1.(CsemC.get_mem) with
-              | Some m => SimMemId.mk m m
-              | _ => SimMemId.mk tgt tgt
-              end).
-      esplits; eauto.
-      * left. econs; eauto; [econs 1|]. symmetry. apply E0_right.
-      * des_ifs.
-      * des_ifs.
-Qed.
-
-Lemma clight1_inj_id
-      (clight: Clight.program)
-  :
-    exists mp,
-      (<<SIM: @ModPair.sim SimMemInjC.SimMemInj SimMemInjC.SimSymbId SoundTop.Top mp>>)
-      /\ (<<SRC: mp.(ModPair.src) = clight.(module1)>>)
-      /\ (<<TGT: mp.(ModPair.tgt) = clight.(module1)>>)
-.
-Proof.
-  admit "this should hold".
-Qed.
-
 Definition match_env (j: meminj) (env_src env_tgt: env) :=
   forall id,
     (<<MAPPED: exists blk_src blk_tgt ty,
@@ -139,6 +72,40 @@ Inductive match_cont (j: meminj): cont -> cont -> Prop :=
   :
     match_cont j (Kcall id fn env_src tenv_src K_src) (Kcall id fn env_tgt tenv_tgt K_tgt)
 .
+
+(* Inductive match_ext_cont: cont -> cont -> Prop := *)
+(* | match_ext_Kstop: *)
+(*     match_ext_cont Kstop Kstop *)
+(* | match_ext_Kseq *)
+(*     stmt K_src K_tgt *)
+(*     (CONT: match_ext_cont K_src K_tgt) *)
+(*   : *)
+(*     match_ext_cont (Kseq stmt K_src) (Kseq stmt K_tgt) *)
+(* | match_ext_Kloop1 *)
+(*     stmt0 stmt1 K_src K_tgt *)
+(*     (CONT: match_ext_cont K_src K_tgt) *)
+(*   : *)
+(*     match_ext_cont (Kloop1 stmt0 stmt1 K_src) (Kloop1 stmt0 stmt1 K_tgt) *)
+(* | match_ext_Kloop2 *)
+(*     stmt0 stmt1 K_src K_tgt *)
+(*     (CONT: match_ext_cont K_src K_tgt) *)
+(*   : *)
+(*     match_ext_cont (Kloop2 stmt0 stmt1 K_src) (Kloop2 stmt0 stmt1 K_tgt) *)
+(* | match_ext_Kswitch *)
+(*     K_src K_tgt *)
+(*     (CONT: match_ext_cont K_src K_tgt) *)
+(*   : *)
+(*     match_ext_cont (Kswitch K_src) (Kswitch K_tgt) *)
+(* | match_ext_Kcall *)
+(*     id fn *)
+(*     env_src env_tgt *)
+(*     tenv_src tenv_tgt *)
+(*     K_src K_tgt *)
+(*     (TENV: match_temp_env inject_id tenv_src tenv_tgt) *)
+(*     (CONT: match_ext_cont K_src K_tgt) *)
+(*   : *)
+(*     match_ext_cont (Kcall id fn env_src tenv_src K_src) (Kcall id fn env_tgt tenv_tgt K_tgt) *)
+(* . *)
 
 Inductive match_states_clight (sm_arg: SimMemInj.t')
   : unit -> state -> state -> SimMemInj.t' -> Prop :=
@@ -192,8 +159,8 @@ Inductive match_states_ext_clight (sm_arg: SimMemExt.t')
     (MWFSRC: m_src = sm0.(SimMemExt.src))
     (MWFTGT: m_tgt = sm0.(SimMemExt.tgt))
     (MWF: Mem.extends m_src m_tgt)
-    (ENV: env_src = env_tgt)
-    (TENV: tenv_src = tenv_tgt)
+    (ENV: match_env inject_id env_src env_tgt)
+    (TENV: match_temp_env inject_id tenv_src tenv_tgt)
     (CONT: match_cont inject_id K_src K_tgt)
   :
     match_states_ext_clight
@@ -229,102 +196,6 @@ Inductive match_states_ext_clight (sm_arg: SimMemExt.t')
       (Returnstate retv_tgt K_tgt m_tgt)
       sm0
 .
-
-Lemma clight2_id
-      (clight: Clight.program)
-  :
-    exists mp,
-      (<<SIM: @ModPair.sim SimMemId.SimMemId SimMemId.SimSymbId SoundTop.Top mp>>)
-      /\ (<<SRC: mp.(ModPair.src) = clight.(module2)>>)
-      /\ (<<TGT: mp.(ModPair.tgt) = clight.(module2)>>)
-.
-Proof.
-  eexists (ModPair.mk _ _ _); s.
-  esplits; eauto. instantiate (1:=tt).
-  econs; ss; i.
-  rewrite SIMSKENVLINK in *.
-  eapply match_states_sim; ss.
-  - apply unit_ord_wf.
-  - eapply SoundTop.sound_state_local_preservation.
-  - instantiate (1:= fun sm_arg _ st_src st_tgt sm0 =>
-                       (<<EQ: st_src = st_tgt>>) /\
-                       (<<MWF: sm0.(SimMemId.src) = sm0.(SimMemId.tgt)>>) /\
-                       (<<STMWF: st_src.(ClightC.get_mem) =
-                                 sm0.(SimMemId.src)>>)).
-    ss. i.
-    destruct args_src, args_tgt, sm_arg. inv SIMARGS; ss; clarify.
-    clear SAFESRC. dup INITTGT. inv INITTGT. ss.
-    eexists. eexists (SimMemId.mk tgt tgt). esplits; eauto; ss.
-  - ii. destruct args_src, args_tgt, sm_arg. inv SIMARGS; ss; clarify.
-  - ii. ss. des. clarify.
-  - i. ss. des. clarify. esplits; eauto.
-    + inv CALLSRC. ss. clarify.
-    + instantiate (1:=top4). ss.
-  - i. clear HISTORY. ss. destruct sm_ret, retv_src, retv_tgt.
-    inv SIMRET. des. ss. clarify. eexists (SimMemId.mk _ _). esplits; eauto.
-    inv AFTERSRC. ss.
-  - i. ss. des. destruct sm0. ss. clarify.
-    eexists (SimMemId.mk (get_mem st_tgt0) (get_mem st_tgt0)).
-    esplits; eauto.
-    inv FINALSRC. ss.
-  - right. ii. des. destruct sm0. ss. clarify. esplits; eauto.
-    + i. exploit H; ss.
-      * econs 1.
-      * i. des; clarify. econs; eauto.
-    + i. exists tt, st_tgt1.
-      eexists (SimMemId.mk (get_mem st_tgt1) (get_mem st_tgt1)).
-      esplits; eauto.
-      left. econs; eauto; [econs 1|]. symmetry. apply E0_right.
-Qed.
-
-Lemma clight2_ext_top
-      (clight: Clight.program)
-  :
-    exists mp,
-      (<<SIM: @ModPair.sim SimMemExt.SimMemExt SimMemExt.SimSymbExtends SoundTop.Top mp>>)
-      /\ (<<SRC: mp.(ModPair.src) = clight.(module2)>>)
-      /\ (<<TGT: mp.(ModPair.tgt) = clight.(module2)>>)
-.
-Proof.
-  admit "this should hold".
-Qed.
-
-Lemma clight2_ext_unreach
-      (clight: Clight.program)
-  :
-    exists mp,
-      (<<SIM: @ModPair.sim SimMemExt.SimMemExt SimMemExt.SimSymbExtends UnreachC.Unreach mp>>)
-      /\ (<<SRC: mp.(ModPair.src) = clight.(module2)>>)
-      /\ (<<TGT: mp.(ModPair.tgt) = clight.(module2)>>)
-.
-Proof.
-  admit "this should hold".
-Qed.
-
-Lemma clight2_inj_id
-      (clight: Clight.program)
-  :
-    exists mp,
-      (<<SIM: @ModPair.sim SimMemInjC.SimMemInj SimMemInjC.SimSymbId SoundTop.Top mp>>)
-      /\ (<<SRC: mp.(ModPair.src) = clight.(module2)>>)
-      /\ (<<TGT: mp.(ModPair.tgt) = clight.(module2)>>)
-.
-Proof.
-  admit "this should hold".
-Qed.
-
-Lemma clight2_inj_drop
-      (clight: Clight.program)
-  :
-    exists mp,
-      (<<SIM: @ModPair.sim SimMemInjC.SimMemInj SimSymbDrop.SimSymbDrop SoundTop.Top mp>>)
-      /\ (<<SRC: mp.(ModPair.src) = clight.(module2)>>)
-      /\ (<<TGT: mp.(ModPair.tgt) = clight.(module2)>>)
-.
-Proof.
-  admit "this should hold".
-Qed.
-
 
 Require Import mktac.
 Require Import IntegersC.
@@ -738,7 +609,7 @@ Section CLIGHTINJ.
       end
     end.
 
-  Lemma free_list_parallel
+  Lemma free_list_inject_parallel
         sm0 locs_src locs_tgt m_src1
         (MWF: SimMemInj.wf' sm0)
         (LOCS: list_forall2 (match_loc (SimMemInj.inj sm0)) locs_src locs_tgt)
@@ -997,7 +868,7 @@ Section CLIGHTINJ.
       + econs; eauto.
       + refl.
 
-    - exploit free_list_parallel; eauto.
+    - exploit free_list_inject_parallel; eauto.
       { eapply blocks_of_env_match; eauto. } i. des.
       esplits.
       + econs 15; eauto.
@@ -1007,7 +878,7 @@ Section CLIGHTINJ.
 
     - cinv MWF. exploit eval_expr_inject; eauto. i. des.
       exploit sem_cast_inject; eauto. i. des.
-      exploit free_list_parallel; eauto.
+      exploit free_list_inject_parallel; eauto.
       { eapply blocks_of_env_match; eauto. } i. des.
       esplits.
       + econs 16; eauto.
@@ -1017,7 +888,7 @@ Section CLIGHTINJ.
           cinv MLE. eapply match_cont_incr; eauto.
       + eauto.
 
-    - cinv MWF. exploit free_list_parallel; eauto.
+    - cinv MWF. exploit free_list_inject_parallel; eauto.
       { eapply blocks_of_env_match; eauto. } i. des.
       esplits.
       + econs 17; eauto.
@@ -1075,3 +946,447 @@ Section CLIGHTINJ.
         eapply set_match_temp_env; eauto.
       + refl.
   Qed.
+
+End CLIGHTINJ.
+
+Section CLIGHTEXT.
+
+  Variable se: Senv.t.
+  Variable ge: genv.
+
+  Definition function_entry_extends
+             (function_entry: genv -> function -> list val -> mem -> env -> temp_env -> mem -> Prop)
+    :=
+      forall
+        fn vs_src vs_tgt m_src0 m_tgt0 en tenv_src m_src1
+        (MWF: Mem.extends m_src0 m_tgt0)
+        (VALS: Val.lessdef_list vs_src vs_tgt)
+        (ENTRY: function_entry ge fn vs_src m_src0 en tenv_src m_src1),
+      exists tenv_tgt m_tgt1,
+        (<<MWF: Mem.extends m_src1 m_tgt1>>) /\
+        (<<TENV: match_temp_env inject_id tenv_src tenv_tgt>>) /\
+        (<<ENTRY: function_entry ge fn vs_tgt m_tgt0 en tenv_tgt m_tgt1>>).
+
+  Variable function_entry: genv -> function -> list val -> mem -> env -> temp_env -> mem -> Prop.
+  Hypothesis FUNCTIONENTRY: function_entry_extends function_entry.
+
+  Lemma alloc_variables_extends idl en_src0 en_tgt0 en_src1 m_src0 m_tgt0 m_src1
+        (ALLOC: alloc_variables ge en_src0 m_src0 idl en_src1 m_src1)
+        (ENV: match_env inject_id en_src0 en_tgt0)
+        (MWF: Mem.extends m_src0 m_tgt0)
+    :
+      exists m_tgt1 en_tgt1,
+        (<<MWF: Mem.extends m_src1 m_tgt1>>) /\
+        (<<ENV: match_env inject_id en_src1 en_tgt1>>) /\
+        (<<ALLOC: alloc_variables ge en_src0 m_tgt0 idl en_src1 m_tgt1>>).
+  Proof.
+    revert m_src0 m_src1 m_tgt0 en_src0 en_tgt0 en_src1 ALLOC ENV MWF. induction idl.
+    - i. inv ALLOC. esplits; eauto.
+      econs; eauto.
+    - i. inv ALLOC.
+      exploit Mem.alloc_extends; eauto; try refl. i. des.
+      exploit IHidl; eauto.
+      { instantiate (1:=PTree.set id (b1, ty) en_tgt0).
+        ii. repeat rewrite PTree.gsspec. des_ifs.
+        left. esplits; ss. } i. des.
+      esplits; eauto.
+      econs; eauto.
+  Qed.
+
+  Lemma match_env_inject_id en
+    :
+      match_env inject_id en en.
+  Proof.
+    ii. destruct (en ! id) eqn:ENV; eauto.
+    destruct p. left. esplits; ss.
+  Qed.
+
+  Lemma function_entry2_extends
+    :
+      function_entry_extends function_entry2.
+  Proof.
+    ii. inv ENTRY.
+    exploit alloc_variables_extends; eauto.
+    { eapply match_env_inject_id. } i. des.
+    exploit bind_parameter_temps_inject; eauto.
+    { eapply create_undef_temps_match. }
+    { eapply val_inject_list_lessdef. eauto. } i. des.
+    esplits; eauto. econs; eauto.
+  Qed.
+
+  Lemma assign_loc_extends ce ty m_src0 m_tgt0 v_src v_tgt m_src1 blk ofs
+        (ASSIGN: assign_loc ce ty m_src0 blk ofs v_src m_src1)
+        (VAL: Val.lessdef v_src v_tgt)
+        (MWF: Mem.extends m_src0 m_tgt0)
+    :
+      exists m_tgt1,
+        (<<ASSIGN: assign_loc ce ty m_tgt0 blk ofs v_tgt m_tgt1>>) /\
+        (<<MWF: Mem.extends m_src1 m_tgt1>>).
+  Proof.
+    inv ASSIGN.
+    - exploit Mem.storev_extends; eauto. i. des.
+      esplits; eauto. econs 1; eauto.
+    - cinv VAL.
+      exploit Mem.loadbytes_extends; eauto. i. des_safe.
+      exploit Mem.storebytes_within_extends; eauto. i. des_safe.
+      esplits; eauto. econs 2; eauto.
+  Qed.
+
+  Lemma bool_val_extends m_src m_tgt ty v_src v_tgt b
+        (VAL: Val.lessdef v_src v_tgt)
+        (MWF: Mem.extends m_src m_tgt)
+        (BVAL: bool_val v_src ty m_src = Some b)
+    :
+      bool_val v_tgt ty m_tgt = Some b.
+  Proof.
+    unfold bool_val in *. cinv VAL; des_ifs; ss; clarify.
+    exploit Mem.weak_valid_pointer_extends; eauto. i. clarify.
+  Qed.
+
+  Lemma sem_unary_operation_extends m_src m_tgt op v_src0 v_tgt0 v_src1 ty
+        (EXT: Mem.extends m_src m_tgt)
+        (VAL: Val.lessdef v_src0 v_tgt0)
+        (SEM: sem_unary_operation op v_src0 ty m_src = Some v_src1)
+    :
+      exists v_tgt1,
+        (<<SEM: sem_unary_operation op v_tgt0 ty m_tgt = Some v_tgt1>>) /\
+        (<<VAL: Val.lessdef v_src1 v_tgt1>>).
+  Proof.
+    destruct op; ss.
+    - unfold sem_notbool, option_map in *. des_ifs_safe.
+      exploit bool_val_extends; eauto.
+      intros BVAL. rewrite BVAL. esplits; eauto.
+    - unfold sem_notint in *. cinv VAL; des_ifs; esplits; eauto.
+    - unfold sem_neg in *. cinv VAL; des_ifs; esplits; eauto.
+    - unfold sem_absfloat in *. cinv VAL; des_ifs; esplits; eauto.
+  Qed.
+
+  Lemma sem_binary_operation_extends ce m_src m_tgt op
+        v_src0 v_tgt0 v_src1 v_tgt1 v_src2 ty0 ty1
+        (SEM: sem_binary_operation ce op v_src0 ty0 v_src1 ty1 m_src = Some v_src2)
+        (EXT: Mem.extends m_src m_tgt)
+        (VAL0: Val.lessdef v_src0 v_tgt0)
+        (VAL1: Val.lessdef v_src1 v_tgt1)
+    :
+      exists v_tgt2,
+        (<<SEM: sem_binary_operation ce op v_tgt0 ty0 v_tgt1 ty1 m_tgt = Some v_tgt2>>) /\
+        (<<VAL: Val.lessdef v_src2 v_tgt2>>).
+  Proof.
+    exploit sem_binary_operation_inj; try eassumption.
+    - instantiate (1:=m_tgt). instantiate (1:=fun b => Some (b, 0)).
+      i. ss. clarify. psimpl.
+      eapply Mem.valid_pointer_extends; eauto.
+    - i. ss. clarify. psimpl. eapply Mem.weak_valid_pointer_extends; eauto.
+    - i. ss. clarify. psimpl. zsimpl.
+      eapply Ptrofs.unsigned_range_2; eauto.
+    - i. ss. clarify. eauto.
+    - eapply val_inject_id; eauto.
+    - eapply val_inject_id; eauto.
+    - i. des. esplits; eauto.
+      eapply val_inject_id; eauto.
+  Qed.
+
+  Lemma sem_cast_extends m_src m_tgt v_src0 v_tgt0 v_src1 ty0 ty1
+        (EXT: Mem.extends m_src m_tgt)
+        (VAL: Val.lessdef v_src0 v_tgt0)
+        (SEM: sem_cast v_src0 ty0 ty1 m_src = Some v_src1)
+    :
+      exists v_tgt1,
+        (<<SEM: sem_cast v_tgt0 ty0 ty1 m_tgt = Some v_tgt1>>) /\
+        (<<VAL: Val.lessdef v_src1 v_tgt1>>).
+  Proof.
+    exploit sem_cast_inj; try eassumption.
+    - instantiate (1:=m_tgt). instantiate (1:=fun b => Some (b, 0)).
+      i. ss. clarify. psimpl. eapply Mem.weak_valid_pointer_extends; eauto.
+    - eapply val_inject_id; eauto.
+    - i. des. esplits; eauto.
+      eapply val_inject_id; eauto.
+  Qed.
+
+  Lemma deref_loc_extends ty m_src m_tgt blk ofs v_src
+        (DEREF: deref_loc ty m_src blk ofs v_src)
+        (EXT: Mem.extends m_src m_tgt)
+    :
+      exists v_tgt,
+        (<<DEREF: deref_loc ty m_tgt blk ofs v_tgt>>) /\
+        (<<VAL: Val.lessdef v_src v_tgt>>).
+  Proof.
+    inv DEREF.
+    - exploit Mem.loadv_extends; eauto. i. des.
+      esplits; eauto. econs 1; eauto.
+    - esplits; eauto. econs 2; eauto.
+    - esplits; eauto. econs 3; eauto.
+  Qed.
+
+  Lemma eval_expr_lvalue_extends en_src en_tgt tenv_src tenv_tgt m_src m_tgt
+        (ENV: match_env inject_id en_src en_tgt)
+        (TENV: match_temp_env inject_id tenv_src tenv_tgt)
+        (EXT: Mem.extends m_src m_tgt)
+    :
+      (forall
+          exp v_src
+          (EVAL: eval_expr ge en_src tenv_src m_src exp v_src),
+          exists v_tgt,
+            (<<EVAL: eval_expr ge en_tgt tenv_tgt m_tgt exp v_tgt>>) /\
+            (<<LESS: Val.lessdef v_src v_tgt>>)) /\
+      (forall
+          exp blk ofs
+          (EVAL: eval_lvalue ge en_src tenv_src m_src exp blk ofs),
+          eval_lvalue ge en_tgt tenv_tgt m_tgt exp blk ofs).
+  Proof.
+    apply eval_expr_lvalue_ind; i; try by (esplits; eauto; econs; eauto).
+    - cinv (TENV id); rewrite H in *; clarify.
+      erewrite val_inject_id in *.
+      esplits; eauto. econs 5; eauto.
+    - des. exploit sem_unary_operation_extends; eauto. i. des.
+      esplits; eauto. econs; eauto.
+    - des. exploit sem_binary_operation_extends; eauto. i. des.
+      esplits; eauto. econs; eauto.
+    - des. exploit sem_cast_extends; eauto. i. des.
+      esplits; eauto. econs; eauto.
+    - des. exploit deref_loc_extends; eauto. i. des.
+      esplits; eauto. econs 12; eauto.
+    - cinv (ENV id); des; clarify. unfold inject_id in *.
+      clarify. econs; eauto.
+    - cinv (ENV id); des; clarify.
+      econs 2; eauto.
+    - des. cinv LESS. econs; eauto.
+    - des. cinv LESS. econs; eauto.
+    - des. cinv LESS. econs; eauto.
+  Qed.
+
+  Lemma eval_expr_extends en_src en_tgt tenv_src tenv_tgt m_src m_tgt
+        (ENV: match_env inject_id en_src en_tgt)
+        (TENV: match_temp_env inject_id tenv_src tenv_tgt)
+        (EXT: Mem.extends m_src m_tgt)
+        exp v_src
+        (EVAL: eval_expr ge en_src tenv_src m_src exp v_src)
+    :
+      exists v_tgt,
+        (<<EVAL: eval_expr ge en_tgt tenv_tgt m_tgt exp v_tgt>>) /\
+        (<<LESS: Val.lessdef v_src v_tgt>>).
+  Proof.
+    eapply eval_expr_lvalue_extends; eauto.
+  Qed.
+
+  Lemma eval_exprlist_extends en_src en_tgt tenv_src tenv_tgt m_src m_tgt tys
+        (ENV: match_env inject_id en_src en_tgt)
+        (TENV: match_temp_env inject_id tenv_src tenv_tgt)
+        (EXT: Mem.extends m_src m_tgt)
+        exps vs_src
+        (EVALS: eval_exprlist ge en_src tenv_src m_src exps tys vs_src)
+    :
+      exists vs_tgt,
+        (<<EVALS: eval_exprlist ge en_tgt tenv_tgt m_tgt exps tys vs_tgt>>) /\
+        (<<LESS: Val.lessdef_list vs_src vs_tgt>>).
+  Proof.
+    revert tys vs_src EVALS TENV EXT. induction exps; i.
+    - inv EVALS. exists []. esplits; eauto. econs; eauto.
+    - inv EVALS. exploit IHexps; eauto. i. des.
+      exploit eval_expr_extends; eauto. i. des.
+      exploit sem_cast_extends; eauto. i. des.
+      exists (v_tgt1 :: vs_tgt). esplits; eauto.
+      econs; eauto.
+  Qed.
+
+  Lemma eval_lvalue_extends en_src en_tgt tenv_src tenv_tgt m_src m_tgt
+        (ENV: match_env inject_id en_src en_tgt)
+        (TENV: match_temp_env inject_id tenv_src tenv_tgt)
+        (EXT: Mem.extends m_src m_tgt)
+        exp blk ofs
+        (EVAL: eval_lvalue ge en_src tenv_src m_src exp blk ofs)
+    :
+      eval_lvalue ge en_tgt tenv_tgt m_tgt exp blk ofs.
+  Proof.
+    exploit eval_expr_lvalue_extends; eauto. i. des. eauto.
+  Qed.
+
+  Lemma free_list_extends_parallel
+        m_src0 m_tgt0 locs m_src1
+        (MWF: Mem.extends m_src0 m_tgt0)
+        (FREE: Mem.free_list m_src0 locs = Some m_src1)
+    :
+      exists m_tgt1,
+        (<<MWF: Mem.extends m_src1 m_tgt1>>) /\
+        (<<FREE: Mem.free_list m_tgt0 locs = Some m_tgt1>>).
+  Proof.
+    revert m_src0 m_tgt0 m_src1 FREE MWF. induction locs; ss.
+    - i. clarify. esplits; eauto.
+    - i. des_ifs_safe.
+      exploit Mem.free_parallel_extends; eauto. i. des.
+      exploit IHlocs; eauto. i. des.
+      esplits; eauto.
+      rewrite H. rewrite FREE0. eauto.
+  Qed.
+
+  Lemma blocks_of_env_ext_match e_src e_tgt
+        (ENV: match_env inject_id e_src e_tgt)
+    :
+      (blocks_of_env ge e_src) = (blocks_of_env ge e_tgt).
+  Proof.
+    exploit PTree.elements_canonical_order.
+    - instantiate (1:= @eq (block * type)).
+      instantiate (1:= e_tgt).
+      instantiate (1:= e_src).
+      i. unfold inject_id in *. destruct (ENV i); des; clarify.
+      esplits; eauto; ss.
+    - i. unfold inject_id in *. destruct (ENV i); des; clarify.
+      esplits; eauto.
+    - intros ALL.
+      unfold blocks_of_env. revert ALL.
+      generalize (PTree.elements e_tgt).
+      generalize (PTree.elements e_src).
+      induction l; ss; i.
+      + inv ALL. econs.
+      + inv ALL. ss. destruct a, b1. ss. des. clarify.
+        des_ifs; ss. f_equal.
+        exploit IHl; eauto.
+  Qed.
+
+  Lemma clight_step_preserve_extension
+        sm_arg u st_src0 st_tgt0 st_src1 sm0 tr
+        (MATCH: match_states_ext_clight sm_arg u st_src0 st_tgt0 sm0)
+        (STEP: step se ge (function_entry ge) st_src0 tr st_src1)
+  :
+    exists st_tgt1 sm1,
+      (<<STEP: step se ge (function_entry ge) st_tgt0 tr st_tgt1>>) /\
+      (<<MATCH: match_states_ext_clight sm_arg u st_src1 st_tgt1 sm1>>).
+  Proof.
+    inv STEP; inv MATCH.
+    - exploit eval_expr_extends; eauto. i. des.
+      exploit eval_lvalue_extends; eauto. i. des.
+      exploit sem_cast_extends; eauto. i. des.
+      exploit assign_loc_extends; eauto. i. des.
+      eexists. eexists (SimMemExt.mk _ _). esplits.
+      + econs 1; eauto.
+      + econs; ss; eauto.
+
+    - exploit eval_expr_extends; eauto. i. des.
+      eexists. eexists (SimMemExt.mk _ _). esplits.
+      + econs 2; eauto.
+      + econs; ss; eauto.
+        eapply set_match_temp_env; eauto.
+        eapply val_inject_id; eauto.
+
+    - exploit eval_exprlist_extends; eauto. i. des.
+      exploit eval_expr_extends; eauto. i. des. esplits.
+      + econs 3; eauto.
+      + econs; eauto. econs; eauto.
+
+    - exploit eval_exprlist_extends; eauto. i. des.
+      exploit external_call_mem_extends; eauto. i. des.
+      eexists. eexists (SimMemExt.mk _ _). esplits.
+      + econs 4; eauto.
+      + econs; ss; eauto. destruct optid; ss.
+        eapply set_match_temp_env; eauto.
+        eapply val_inject_id; eauto.
+
+    - esplits.
+      + econs 5; eauto.
+      + econs; eauto. econs; eauto.
+
+    - inv CONT. esplits.
+      + econs 6; eauto.
+      + econs; eauto.
+
+    - inv CONT. esplits.
+      + econs 7; eauto.
+      + econs; eauto.
+
+    - inv CONT. esplits.
+      + econs 8; eauto.
+      + econs; eauto.
+
+    - exploit eval_expr_extends; eauto. i. des.
+      exploit bool_val_extends; eauto. i. esplits.
+      + econs 9; eauto.
+      + econs; eauto.
+
+    - esplits.
+      + econs 10; eauto.
+      + econs; eauto. econs; eauto.
+
+    - inv CONT. esplits.
+      + econs 11; eauto.
+      + econs; eauto. econs; eauto.
+
+    - inv CONT. esplits.
+      + econs 12; eauto.
+      + econs; eauto.
+
+    - inv CONT. esplits.
+      + econs 13; eauto.
+      + econs; eauto.
+
+    - inv CONT. esplits.
+      + econs 14; eauto.
+      + econs; eauto.
+
+    - exploit free_list_extends_parallel; eauto. i. des.
+      erewrite blocks_of_env_ext_match in *; eauto.
+      eexists. eexists (SimMemExt.mk _ _). esplits.
+      + econs 15; eauto.
+      + econs; ss; eauto. eapply call_cont_match; eauto.
+
+    - exploit eval_expr_extends; eauto. i. des.
+      exploit sem_cast_extends; eauto. i. des.
+      erewrite blocks_of_env_ext_match in *; eauto.
+      exploit free_list_extends_parallel; eauto. i. des.
+      eexists. eexists (SimMemExt.mk _ _). esplits.
+      + econs 16; eauto.
+      + econs; ss; eauto. eapply call_cont_match; eauto.
+
+    - exploit free_list_extends_parallel; eauto. i. des.
+      erewrite blocks_of_env_ext_match in *; eauto.
+      eexists. eexists (SimMemExt.mk _ _). esplits.
+      + econs 17; eauto.
+        unfold is_call_cont in *. destruct CONT; clarify.
+      + econs; ss; eauto.
+
+    - exploit eval_expr_extends; eauto. i. des.
+      assert (SWITCH: sem_switch_arg v_tgt (typeof a) = Some n).
+      { unfold sem_switch_arg in *. inv LESS; ss; clarify; des_ifs. }
+      eexists. eexists (SimMemExt.mk _ _). esplits.
+      + econs 18; eauto.
+      + econs; ss; eauto. econs; eauto.
+
+    - inv CONT. esplits.
+      + econs 19; eauto.
+      + econs; eauto.
+
+    - inv CONT. esplits.
+      + econs 20; eauto.
+      + econs; eauto.
+
+    - esplits.
+      + econs 21; eauto.
+      + econs; eauto.
+
+    - exploit find_label_match; eauto.
+      { eapply call_cont_match; eauto. } i. des.
+      esplits.
+      + econs 22; eauto.
+      + econs; eauto.
+
+    - cinv INJ; clarify.
+      exploit FUNCTIONENTRY; eauto. i. des. clarify.
+      eexists. eexists (SimMemExt.mk _ _). esplits.
+      + econs 23; eauto.
+      + econs; ss; eauto.
+        eapply match_env_inject_id; eauto.
+
+    - cinv INJ; clarify.
+      exploit external_call_mem_extends; eauto. i. des.
+      eexists. eexists (SimMemExt.mk _ _). esplits.
+      + econs 24; eauto.
+      + econs; ss; eauto.
+
+    - inv CONT.
+      esplits.
+      + econs 25; eauto.
+      + econs; eauto. destruct optid; ss.
+        eapply set_match_temp_env; eauto.
+        eapply val_inject_id. eauto.
+  Qed.
+
+End CLIGHTEXT.
